some progress on callQuery under Jon's supervision

concurrency/hack-hash-table/Impl.i.dfy
@@ -3,7 +3,7 @@ include "HTResource.i.dfy"
 include "Main.s.dfy"
 
 module HTMutex refines AbstractMutex {
-  import HTResource
+  import opened HTResource
 
   type ConstType = int  // the row in the hash table protected by this mutex
 
@@ -12,10 +12,8 @@ module HTMutex refines AbstractMutex {
       /* ghost */ linear resource: HTResource.R)
 
   predicate Inv(k: ConstType, v: ValueType) {
-    && v.resource.R?
-    && 0 <= k < |v.resource.table|
-    && v.resource.table[k].value.entry == v.entry
-    && v.resource.table[k].value.state.Free?
+    && 0 <= k < FixedSize()
+    && v.resource == singletonEntry(k as nat, Info(v.entry, Free))
   }
 }
 
@@ -24,10 +22,12 @@ module Impl refines Main {
   import opened NativeTypes
   import opened HTMutex
   import opened HTResource
+  import opened KeyValueType
 
-  type Object = seq<HTMutex.Mutex>
-  predicate Inv(o: Object) {
-    |o| == HTResource.FixedSize()
+  type MutexTable = seq<HTMutex.Mutex>
+  predicate Inv(o: MutexTable) {
+    && |o| == HTResource.FixedSize()
+    && (forall i: nat | i < |o| :: o[i].constant() == i)
   }
 
   predicate Init(s: ARS.R) {
@@ -50,34 +50,89 @@ module Impl refines Main {
   }
 
   method init(linear in_r: ARS.R)
-  returns (o: Object)
-  //requires ARS.Init(i)
+  returns (o: MutexTable, linear out_r: ARS.R)
+  // requires ARS.Init(i)
   ensures Inv(o)
+  ensures out_r == unit()
   {
-    var remaining_r := in_r;
+    linear var remaining_r := in_r;
     o := [];
     var i:uint32 := 0;
     while i < FixedSizeImpl()
+      invariant i as int == |o| <= FixedSize()
       invariant forall j:nat | j<i as int :: && o[j].constant() as int == j
+      invariant remaining_r.R?
+      invariant remaining_r.tickets == multiset{}
+      invariant remaining_r.stubs == multiset{} 
+      invariant forall k:nat | k < i as int :: remaining_r.table[k].None?
+      invariant forall l:nat | i as int <= l < |remaining_r.table| :: remaining_r.table[l] == Some(Info(Empty, Free))
     {
       ghost var splitted := Split(remaining_r, i as int);
-      var remaining_r', ri := ARS.split(remaining_r, splitted.r', splitted.ri);
-      remaining_r := remaining_r';
+      linear var ri;
+      remaining_r, ri := ARS.split(remaining_r, splitted.r', splitted.ri);
       var m := new_mutex(i as int, Value(Empty, ri));
       o := o + [m];
       i := i + 1;
     }
+
+    out_r := remaining_r;
+
+    assert forall i:nat | i < FixedSize() :: out_r.table[i].None?;
+    assert out_r == unit();
   }
 
-  method call_Insert(o: Object, input: Ifc.Input, rid: int, /*ghost*/ linear insert_ticket: ARS.R)
+  method callQuery(mt: MutexTable, input: Ifc.Input, rid: int, /*ghost*/ linear query_ticket_r: ARS.R)
+  returns (output: Ifc.Output, linear out_r: ARS.R)
+    requires Inv(mt)
+    requires input.QueryInput?
+    requires query_ticket_r.R?
+    requires forall i:nat | i < |query_ticket_r.table| :: query_ticket_r.table[i].None?
+    requires query_ticket_r.tickets == multiset { Ticket(rid, input) }
+    requires query_ticket_r.stubs == multiset { }
+    // ensures out_r == ARS.output_stub(rid, output)
+  {
+    var query_ticket := Ticket(rid, input);
+    var key := input.key;
+    var h := hash(key);
+    linear var row: HTMutex.ValueType := HTMutex.acquire(mt[h]);
+
+    linear var Value(entry, row_r) := row;
+    linear var r := ARS.join(query_ticket_r, row_r);
+    ghost var r1 := singletonEntry(h as nat, Info(entry, Querying(query_ticket.rid, query_ticket.input.key)));
+    assert UpdateStep(r, r1, ProcessQueryTicketStep(query_ticket)); // observe
+    r := easy_transform(r, r1);
+
+    if entry.Empty? {
+      output := MapIfc.QueryOutput(NotFound);
+      ghost var stub := Stub(rid, output);
+      ghost var r2 := R(singletonTable(h as nat, Info(entry, Free)), multiset{}, multiset{stub}); 
+      assert UpdateStep(r, r2, QueryNotFoundStep(h as nat)); // observe
+      r := easy_transform(r, r2);
+
+      linear var rmutex;
+
+      ghost var left := ARS.output_stub(rid, output);
+      ghost var right := singletonEntry(h as nat, Info(entry, Free));
+
+      r, rmutex := ARS.split(r, left, right);
+      release(mt[h], Value(entry, rmutex));
+
+      assert r == ARS.output_stub(rid, output);
+    }
+
+    out_r := r;
+  }
+
+  method call_Insert(o: MutexTable, input: Ifc.Input, rid: int, /*ghost*/ linear insert_ticket: ARS.R)
   returns (output: Ifc.Output, linear out_r: ARS.R)
     requires forall i:nat | i < |insert_ticket.table| :: insert_ticket.table[i].None?
     requires insert_ticket.tickets == multiset { Ticket(rid, input) }
     requires insert_ticket.stubs == multiset { }
   {
+    out_r := insert_ticket;
   }
 
-  method call(o: Object, input: Ifc.Input,
+  method call(o: MutexTable, input: Ifc.Input,
       rid: int, linear in_r: ARS.R)
   returns (output: Ifc.Output, linear out_r: ARS.R)
   //requires Inv(o)
@@ -89,28 +144,20 @@ module Impl refines Main {
     var the_ticket :| the_ticket in in_r.tickets;
 
     if the_ticket.input.QueryInput? {
-      //call_Query(o, input, rid, in_r);
+      output, out_r := callQuery(o, input, rid, in_r);
     } else if the_ticket.input.InsertInput? {
+      assume false;
       output, out_r := call_Insert(o, input, rid, in_r);
     } else if the_ticket.input.RemoveInput? {
+      assume false;
+      out_r := in_r;
       // call_Remove(o, input, rid, in_r);
     } else {
+      out_r := in_r;
       assert false;
     }
 
-    match the_ticket.input {
-      case QueryInput(key) => {
-        var h := hash(key);
-        linear var row: HTMutex.ValueType := HTMutex.acquire(o[h]);
-        linear var Value(entry_r, row_r) := row;
-        linear var r := ARS.join(in_r, row_r);
-
-      }
-      case InsertInput(key, value) => { assume false; }
-      case RemoveInput(key) => assume false; { }
-    }
-
-//    linear var Value(sugar, butter, pantry_object) := p;
+//    linear var Value(sugar, butter, pantry_MutexTable) := p;
 //
 //    sugar := sugar + input.sugar;
 //    butter := butter + input.butter;
@@ -123,7 +170,7 @@ module Impl refines Main {
 //    output := Ifc.Output(num_batches * 6);
 //
 //    linear var cookies, new_pantry := CookieResource.do_tr( // ghost
-//        ticket, pantry_object, CookieResource.Ticket(rid, input), num_batches);
+//        ticket, pantry_MutexTable, CookieResource.Ticket(rid, input), num_batches);
 //
 //    stub := cookies;
 //
